end-to-end examples in examples/examples.sml

examples/dev/sw/examples/examples.sml
@@ -1,338 +1,135 @@
-(* 
- loadPath := ".." :: !loadPath;
-*)
+(*---------------------------------------------------------------------------------*)
+(*      Simple Examples                                                            *) 
+(*      No precedure call is presented in these examples                           *)
+(*---------------------------------------------------------------------------------*)
 
 use "compiler";
 
-(*---------------------------------------------------------------------------*)
-(* Example 1: A simple program						     *)
-(* It implements the addition of two word32s                                 *)
-(*---------------------------------------------------------------------------*)
+use "mechReasoning";
 
-val test1_def = Define
-  `test1 (t1:word32,t2:word32) =
-            (let k1 = t1 + t2 in
-	     let k2 = t1 - t2 in
-                (k1,k2)
-            )
-    `;
+(*---------------------------------------------------------------------------------*)
+(*      Single Blocks                                                              *)
+(*      The ShiftXor procedure appearing in TEA                                    *)
+(*---------------------------------------------------------------------------------*)
+
+val ShiftXor_def =
+ Define
+   `ShiftXor (x,s,k0,k1) = ((x << 4) + k0) # (x + s) # ((x >> 5) + k1)`;
+
 (*
-  Name              : test1
-  Arguments         : r0 r1 
-  Modified Registers: r0 r2 
-  Returns           : r2 r0 
-  Body: 
-    0:          mov     ip, sp
-    1:          stmfd   sp!, {fp,ip,lr,pc}
-    2:          sub     fp, ip, #1i
-    3:          add     r2, r0, r1
-    4:          sub     r0, r0, r1
-    5:          sub     sp, fp, #3i
-    6:          ldmfd   sp, {fp,sp,pc}
+ pp_compile ShiftXor_def;
 
-  val env1 = toANF [] test1_def;
-  val arm1 = compileEnv env1;
-
-  set_goal ([], simT (mk_ARM arm1));
-  e (PRE_TAC);
-
-  val test1'_def = Define
-    `test1' [t1; t2] =
-            (let k1 = t1 + t2 in
-             let k2 = t1 - t2 in
-                [k1; k2]
-            )
-    `;
-
-
-  val (_,_, args,stms,outs,_) = hd (#1 arm1);
-  val th1 = hd (sim_to_n [6])
-  val (instM, s0) =  get_instM_state (#2 (top_goal()));
-  val s1 = rhs (concl th1);
-   
-  val p1 = mk_Pd ([], (args,``test1'``,outs)) (s0,s1);
-
-  val result0 = SIMP_RULE finmap_ss [] (EVAL p1);	(* Get the predicate	*)
-  val result1 = REWRITE_RULE [GSYM th1] result0;
+|- !st.
+          get_st
+            (run_arm
+               [((LSL,NONE,F),SOME (REG 4),[REG 0; WCONST 4w],NONE);
+                ((ADD,NONE,F),SOME (REG 2),[REG 4; REG 2],NONE);
+                ((ADD,NONE,F),SOME (REG 1),[REG 0; REG 1],NONE);
+                ((EOR,NONE,F),SOME (REG 1),[REG 2; REG 1],NONE);
+                ((ASR,NONE,F),SOME (REG 0),[REG 0; WCONST 5w],NONE);
+                ((ADD,NONE,F),SOME (REG 0),[REG 0; REG 3],NONE);
+                ((EOR,NONE,F),SOME (REG 0),[REG 1; REG 0],NONE)]
+               ((0,0w,st),{}))<MR R0> =
+          ShiftXor (st<MR R0>,st<MR R1>,st<MR R2>,st<MR R3>))
 *)
-  
-  val env1 = toANF [] test1_def;
-  val arm1 = compileEnv env1;
-  
-  val test1_CORRECT = prove (
-      simT (mk_ARM arm1),
-      SEQ_TAC [test1_def]
+
+(*---------------------------------------------------------------------------------*)
+(*      Single Conditional Jump                                                    *)
+(*---------------------------------------------------------------------------------*)
+
+val f1_def = Define `
+    f1 (a,b) = if a = 1w then b else a + b`;
+
+(*
+ pp_compile f1_def;
+
+|- !st.
+          get_st
+            (run_arm
+               [((CMP,NONE,F),NONE,[REG 0; WCONST 1w],NONE);
+                ((B,SOME EQ,F),NONE,[],SOME (POS 3));
+                ((ADD,NONE,F),SOME (REG 1),[REG 0; REG 1],NONE);
+                ((B,SOME AL,F),NONE,[],SOME (POS 1))]
+               ((0,0w,st),{}))<MR R1> =
+          f1 (st<MR R0>,st<MR R1>))
+
+*)
+
+(*---------------------------------------------------------------------------------*)
+(*      Tail Recusive Functions                                                    *)
+(*      Factorial Function. Form: SC (TR, BLK)                                     *) 
+(*---------------------------------------------------------------------------------*)
+
+val fact_def = Define `
+   fact (x:DATA,a) = if x=0w then a else fact(x-1w,x*a)`;
+
+val fact_thm = Q.store_thm (
+   "fact_thm",
+   `fact = (\(x,a).a) o (WHILE ($~ o (\(x,a).x = 0w)) (\(x,a).(x-1w,x*a)))`,
+   SIMP_TAC std_ss [FUN_EQ_THM, FORALL_PROD] THEN
+   HO_MATCH_MP_TAC (fetch "-" "fact_ind") THEN
+   REPEAT STRIP_TAC THEN
+   ONCE_REWRITE_TAC [fact_def, WHILE] THEN
+   RW_TAC std_ss []
   );
 
-  val test1'_def = Define
-  `test1' [t1; t2] =
-            (let k1 = t1 + t2 in
-             let k2 = t1 - t2 in
-                [k1; k2]
-            )
-    `;
-
-
-(*---------------------------------------------------------------------------*)
-(* Example 2: A functions calls another function                             *)
-(* The proving is performed by "unrolling" the callee                        *)
-(*---------------------------------------------------------------------------*)
-
-val test2_def = Define
-  `test2 (t1:word32,t2:word32) =
-            (let (k1,k2) = test1 (t1,t2) in
-             let k3 = UNCURRY $* (k1,k2) in
-                k3
-            )
-    `;
-
-(******************************************************************
-  Name              : test2
-  Arguments         : r0 r1 
-  Modified Registers: r0 r1 
-  Returns           : r0 
-  Body: 
-    0:          mov     ip, sp
-    1:          stmfd   sp!, {fp,ip,lr,pc}
-    2:          sub     fp, ip, #1i
-    3:          sub     sp, sp, #2i
-    4:          stmfd   sp!, {r0,r1}
-    5:          bl      + (7)
-    6:          add     sp, sp, #2i
-    7:          ldmfd   sp, {r1,r0}
-    8:          add     sp, sp, #2i
-    9:          mul     r0, r1, r0
-   10:          sub     sp, fp, #3i
-   11:          ldmfd   sp, {fp,sp,pc}
-  *****************************************************************
-  Name              : test1
-  Arguments         : r0 r1 
-  Modified Registers: r0 r2 
-  Returns           : r2 r0 
-  Body: 
-   12:          mov     ip, sp
-   13:          stmfd   sp!, {r0,r1,r2,ip,fp,ip,lr,pc}
-   14:          sub     fp, ip, #1i
-   15:          ldmfd   ip, {r0,r1}
-   16:          add     ip, ip, #2i
-   17:          add     r2, r0, r1
-   18:          sub     r0, r0, r1
-   19:          add     sp, fp, #5i
-   20:          stmfd   sp!, {r2,r0}
-   21:          sub     sp, fp, #7i
-   22:          ldmfd   sp, {r0,r1,r2,ip,fp,sp,pc}
-
-  or,
-
-  print_structure := false
- 
-  *****************************************************************
-  Name              : test2
-  Arguments         : r0 r1 
-  Modified Registers: r0 r1 
-  Returns           : r0 
-  Body: 
-    0:          mov     ip, sp
-    1:          stmfd   sp!, {fp,ip,lr,pc}
-    2:          sub     fp, ip, #1i
-    3:          sub     sp, sp, #2i
-    4:          stmfd   sp!, {r0,r1}
-    5:          bl      + (7)
-    6:          add     sp, sp, #2i
-    7:          ldmfd   sp, {r1,r0}
-    8:          add     sp, sp, #2i
-    9:          mul     r0, r1, r0
-   10:          sub     sp, fp, #3i
-   11:          ldmfd   sp, {fp,sp,pc}
-   12:          mov     ip, sp
-   13:          stmfd   sp!, {r0,r1,r2,ip,fp,ip,lr,pc}
-   14:          sub     fp, ip, #1i
-   15:          ldmfd   ip, {r0,r1}
-   16:          add     ip, ip, #2i
-   17:          add     r2, r0, r1
-   18:          sub     r0, r0, r1
-   19:          add     sp, fp, #5i
-   20:          stmfd   sp!, {r2,r0}
-   21:          sub     sp, fp, #7i
-   22:          ldmfd   sp, {r0,r1,r2,ip,fp,sp,pc}
-*)
-
-  val arm2 = link2 test2_def;
-
-  val test2_CORRECT = prove (
-      simT (mk_ARM arm2),
-      SEQ_TAC [test1_def, test2_def]  
-  );
-
-
-
-(*---------------------------------------------------------------------------*)
-(* Example 3: Conditional Jumps                                              *)
-(*                                  					     *)
-(*---------------------------------------------------------------------------*)
-
-
-
-(*---------------------------------------------------------------------------*)
-(* Example 4: Tail Recursive Functions					     *)
-(* This example works on the Factorial Function                              *)
-(*---------------------------------------------------------------------------*)
-
-val (f6_def, f6_ind) = Defn.tprove
- (Hol_defn
-   "f6"
-   `f6 (x,a) = if x=0w then a else f6(x-1w,x*a)`,
-  WF_REL_TAC `measure (w2n o FST)` THEN METIS_TAC [WORD_PRED_THM] );
-
-(******************************************************************
-  Name              : f6
-  Arguments         : r0 r1 
-  Modified Registers: r0 r2 r3 
-  Returns           : r0 
-  Body: 
-    0:          mov     ip, sp
-    1:          stmfd   sp!, {fp,ip,lr,pc}
-    2:          sub     fp, ip, #1i
-    3:          cmp     r0, #0iw
-    4:          beq     + (7)
-    5:          sub     r3, r0, #1iw
-    6:          mul     r2, r0, r1
-    7:          stmfd   sp!, {r3,r2}
-    8:          ldmfd   sp, {r0,r1}
-    9:          add     sp, sp, #2i
-   10:          bal     - (7)
-   11:          mov     r0, r1
-   12:          sub     sp, fp, #3i
-   13:          ldmfd   sp, {fp,sp,pc}
-
-    val env6 = toANF [] f6_def;
-    val arm6 = compileEnv env6;
-	
-    simT (mk_ARM arm6);
-
-
-  The proof:
-
-val fact_tac = 
-
-  REWRITE_TAC [read_thm] THEN
-  REPEAT STRIP_TAC THEN
-
-        (*  Process the first three instructions :
-		    0:          mov     ip, sp
-		    1:          stmfd   sp!, {fp,ip,lr,pc}
-    		    2:          sub     fp, ip, #1
-        *)
-
-  `?pc' cpsr' regs' mems'. run 3 (instB,16) (pc0,cpsr0,regs0,mems0) = (pc',cpsr',regs',mems')` 
-		by METIS_TAC [ABS_PAIR_THM] THEN
-  `terminated (instB,16) (pc',cpsr',regs',mems')` by METIS_TAC [TERMINATED_THM] THEN
-  `terRun (instB,16) (0,cpsr0,regs0,mems0) = terRun (instB,16) (pc',cpsr',regs',mems')` by METIS_TAC [TERRUN_THM] THEN
-  ASM_REWRITE_TAC [] THEN 
-
-  Q.PAT_ASSUM `run 3 (instB,16) x = y` MP_TAC THEN    
-  NTAC 3 ONE_STEP_TAC THEN
-  REWRITE_TAC [run_def] THEN STRIP_TAC THEN 
-
-  POP_ASSUM (ASSUME_TAC o SYM) THEN 
-  FULL_SIMP_TAC std_ss [] THEN
-  REPEAT VAR_EQ_TAC
-
-  	(*  Process the recursive body			*)
-
-  `!cpsr mems. ?k. let (pc',cpsr',regs',mems') = run k (instB,16) (3,cpsr,
-				(\k. k = 15 => 3w | k = 11 => 99w | k = 13 => 96w | k = 12 => 100w | regs0 k), mems) in
-	   			(pc' = 14) /\  (regs' 0 = f6(regs0 0,regs0 1)) /\ 
-	   			(regs' 11 = 99w) /\ (regs' 12 = 100w) /\ (regs' 13 = 96w)` by ALL_TAC THENL [
-
-	NTAC 5 (POP_ASSUM (K ALL_TAC)) THEN	
-	Induct_on `w2n (regs0 0)` THEN REPEAT STRIP_TAC THENL [
-
-		(* Basic case					*)
-
-		`regs0 0 = n2w 0` by METIS_TAC [w2n_ELIM] THEN
-		Q.PAT_ASSUM  `0 = i` (K ALL_TAC) THEN
-		Q.EXISTS_TAC `4` THEN 
-		NTAC 4 ONE_STEP_TAC THEN REWRITE_TAC [Once f6_def, run_def] THEN
-		RW_TAC list_ss [ABS_PAIR_THM],
-
-                (* Inductive case                                   *)
-
-		FULL_SIMP_TAC list_ss [GSYM RIGHT_FORALL_IMP_THM] THEN
-		`?pc1 cpsr1 regs1 mems1. run 10 (instB,16) (3,cpsr,(\k. k = 15 => 3w | k = 11 => 99w | k = 13 => 96w | k 
-					= 12 => 100w | regs0 k),mems) = (pc1,cpsr1,regs1,mems1)`
-                        by METIS_TAC [ABS_PAIR_THM] THEN
-		PAT_ASSUM ``!regs01 cpsr mems.x`` (ASSUME_TAC o Q.SPECL [`regs1`,`cpsr1`,`mems1`]) THEN 
-		FULL_SIMP_TAC list_ss [GSYM RIGHT_EXISTS_IMP_THM] THEN
- 
-		Q.EXISTS_TAC `10 + k` THEN REWRITE_TAC [RUN_THM_1] THEN 
-		Q.ABBREV_TAC `runf = run k (instB,16)` THEN ASM_REWRITE_TAC [] THEN 
-
-		IMP_RES_TAC WORD_IND_LEM THEN
-		Q.PAT_ASSUM `run 10 (instB,16) x = y` (MP_TAC) THEN
-		NTAC 10 ONE_STEP_TAC THEN
-		REWRITE_TAC [Once run_def] THEN STRIP_TAC THEN
-
-		PAT_ASSUM (Term `v = w2n (regs0 0 - 1w)`) (ASSUME_TAC o WORD_RULE) THEN
-		`v = w2n (regs1 0)` by RW_TAC list_ss [] THEN reduceLib.REDUCE_TAC THEN
-		FULL_SIMP_TAC list_ss [ABS_PAIR_THM] THEN 
-
-		`(\k1. k1 = 15 => n2w pc1 | k1 = 11 => 99w | k1 = 13 => 96w | k1 = 12 => 100w | regs1 k1) = regs1` by 
 (*
-REPEAT VAR_EQ_TAC THEN REPEAT (POP_ASSUM (K ALL_TAC))
-THEN SIMP_TAC std_ss [FUN_EQ_THM] 
-THEN GEN_TAC THEN 
-REPEAT (COND_CASES_TAC THEN TRY (VAR_EQ_TAC THEN REDUCE_TAC))
-THEN REWRITE_TAC []
-*)
-			RW_TAC arith_ss [FUN_EQ_THM] THENL [
-				NTAC 6 (POP_ASSUM (K ALL_TAC)) THEN RW_TAC arith_ss [] THEN
-				FULL_SIMP_TAC arith_ss [],  
+  val spec0 = get_spec fact_def;
+  val spec1 = SIMP_RULE std_ss [GSYM fact_thm] spec0;
+  val spec2 = f_correct spec1;
 
-			REWRITE_TAC [Once f6_def] THEN
-			WORD_TAC THEN
-			`(regs1 0 = regs0 0 + 4294967295w) /\ (regs1 1 = regs0 0 * regs0 1)` by RW_TAC arith_ss [] THEN
-			FULL_SIMP_TAC list_ss [ABS_PAIR_THM, LET_THM]
-			]
-		],
-	
-	(*  Process the last two instructions :
-		  14:          sub     sp, fp, #2
-   		  15:          ldmfd   sp, {fp,sp,pc}
-	*)
-
-	POP_ASSUM (STRIP_ASSUME_TAC o REWRITE_RULE [LET_THM] o (Q.SPECL [`cpsr0`, `(\addr. addr = 97 => regs0 11
-             				| addr = 98 => 100w
-               				| addr = 99 => 16w | addr = 100 => 1w | mems0 addr)`])) THEN
-	Q.PAT_ASSUM `terminated (instB,16) (pc0,cpsr0,regs0,mems0)` (K ALL_TAC) THEN 
-	IMP_RES_TAC (Q.SPEC `k` TERRUN_THM) THEN
-	POP_ASSUM (ASSUME_TAC o Q.SPEC `k`) THEN 
-  	ONCE_ASM_REWRITE_TAC [] THEN POP_ASSUM (K ALL_TAC) THEN	
-
-        `?pc1 cpsr1 regs1 mems1. run k (instB,16)
-               (3,cpsr0, (\k. k = 15 => 3w | k = 11 => 99w | k = 13 => 96w | k = 12 => 100w | regs0 k),
-                (\addr. addr = 97 => regs0 11 | addr = 98 => 100w | addr = 99 => 16w | addr = 100 => 1w | mems0 addr)) 
-			= (pc1,cpsr1,regs1,mems1)` by METIS_TAC [ABS_PAIR_THM] THEN
-	`terminated (instB,16) (pc1,cpsr1,regs1,mems1)` by METIS_TAC [TERMINATED_THM] THEN
-	FULL_SIMP_TAC list_ss [] THEN
-	`terRun (instB,16) (14,cpsr1,regs1,mems1) =
-           terRun (instB,16) (run 2 (instB,16) (pc1,cpsr1,regs1,mems1))` by METIS_TAC [TERRUN_THM] THEN
-  	ONCE_ASM_REWRITE_TAC [] THEN
-  	POP_ASSUM (K ALL_TAC) THEN
-  	NTAC 2 ONE_STEP_TAC THEN
-  	RW_TAC std_ss [run_def, TERRUN_STOP]
-    ] 		
-
+   |- !st.
+         get_st
+           (run_arm
+              [((CMP,NONE,F),NONE,[REG 0; WCONST 0w],NONE);
+               ((B,SOME EQ,F),NONE,[],SOME (POS 6));
+               ((SUB,NONE,F),SOME (REG 3),[REG 0; WCONST 1w],NONE);
+               ((MUL,NONE,F),SOME (REG 2),[REG 0; REG 1],NONE);
+               ((MOV,NONE,F),SOME (REG 0),[REG 3],NONE);
+               ((MOV,NONE,F),SOME (REG 1),[REG 2],NONE);
+               ((B,SOME AL,F),NONE,[],SOME (NEG 6));
+               ((MOV,NONE,F),SOME (REG 2),[REG 1],NONE)]
+              ((0,0w,st),{}))<MR R2> =
+         fact (st<MR R0>,st<MR R1>) 
 *)
 
-(*---------------------------------------------------------------------------*)
-(* Example 5: Calling a recursive function				     *) 
-(* In this example, the Factorial Function is called                         *)
-(*---------------------------------------------------------------------------*)
+(*---------------------------------------------------------------------------------*)
+(*      Sequential Compositions                                                    *)
+(*      This example has the form SC (BLK, CJ)                                     *)
+(*---------------------------------------------------------------------------------*)
+
+val f2_def = Define `
+    f2 (a,b) = let c = a + 1w in
+               if a = 1w then c else c + b`;
+
+(*
+ pp_compile f2_def;
+
+ |- !st.
+          get_st
+            (run_arm
+               [((ADD,NONE,F),SOME (REG 2),[REG 0; WCONST 1w],NONE);
+                ((CMP,NONE,F),NONE,[REG 0; WCONST 1w],NONE);
+                ((B,SOME EQ,F),NONE,[],SOME (POS 3));
+                ((ADD,NONE,F),SOME (REG 2),[REG 2; REG 1],NONE);
+                ((B,SOME AL,F),NONE,[],SOME (POS 1))]
+               ((0,0w,st),{}))<MR R2> =
+          f2 (st<MR R0>,st<MR R1>))
+*)
 
 
-val f7_def = Define
-   `f7 x =  
-	let t = f6 (x-1w, 1w) in
-	let k = t + t in
-	k`;
+
+
+(* A more complicated SC example.  Form: SC (BLK, SC (CJ, BLK))         *)
+(* The ANF conversion seems wrong ???                                   *)
+
+val f3_def = Define `
+    f3 (a,b) = let c = a + 1w in
+               let d = if a = 1w then b else a + b in
+               let e = c - d in
+               e 
+`;
+
+(*
+*)
+
